\section{Laurent Series}

\begin{defn}[Laurent Series]
A \emph{Laurent series} is a series of the form
$$
\sum_{n=-\infty}^\infty a_n z^n, \quad a_n \in \mathbb{C}
$$
which converges if both
$$
\sum_{n=0}^\infty a_n z^n
$$
and
\begin{align*}
   \sum_{n=-\infty}^{-1} a_n z^n
&= \sum_{m=1}^\infty a_{-m} z^{-m} \\
&= \sum_{m=1}^\infty a_{-m} \left(\frac{1}{z}\right)^m.
\end{align*}
\end{defn}

Suppose $\sum a_n z^n$ has radius $R_+$ and
$\sum a_{-m} w^m$ is $R_-$. Then the Laurent series
converges when $|z| < R_+$ and $\left|\frac{1}{z}\right| < R_-$,
i.e. $\frac{1}{R_-} < |z| < R_+$. Therefore the series converges
on an annulus.

Let
$$
f(z) = \sum_{n=-\infty}^\infty a_n z^n = f_+(z) + f_-(z)
$$
on $A$ where
$$
f_-(z) = \sum_{n=-\infty}^{-1} a_n z^n = g\left(\frac{1}{z}\right)
$$
and
$$
g(w) = \sum_{m=1}^\infty a_{-m} w^m.
$$
Then $f_+$ is holomorphic on $\{ |z| < R_+ \}$ and
$g$ is holomorphic on $\{ |z| < R_- \}$, so
$f$ is holomorphic on this annulus. Furthermore
$$
  f^\prime(z)
= \sum_{m=1}^\infty n a_n z^{n-1}
+ f_-^\prime(z)
$$
where
\begin{align*}
   f_-^\prime(z)
&= \sum_{m=1}^\infty
     m a_{-m}
     \left(\frac{1}{z}\right)^{m-1}
     \frac{-1}{z^2} \\
&= \sum_{m=1}^\infty (-m) a_{-m} z^{-(m+1)} \\
&= \sum_{n=-\infty}^{-1} n a_n z^{n-1}
\end{align*}
so that
$$
f^\prime(z) = \sum_{n=-\infty}^\infty n a_n z^{n-1}
$$
on the annulus $A$.

\begin{theorem}
Let $0 \leq r < R \leq \infty$. Suppose that $f$ is holomorphic
on the annulus $A(0, r, R)$. Then $f$ has a Laurent series expansion
where
$$
a_n = \frac{1}{2 \pi i} \int_{|z| = t} \frac{f(z)}{z^{n+1}} \dif z
$$
for $n \in \mathbb{Z}$, $t \in (r, R)$.
\end{theorem}

\begin{proof}
Observe that the value of $a_n$ does not depend on the choice of $t$.
Recall that
$$
\frac{1}{1 - z} = \sum_{n=0}^\infty z^n, \quad |z| < 1.
$$
For $|z| < |z_0|$, $\left|\frac{z}{z_0}\right| < 1$ so that
\begin{align*}
   \frac{1}{z - z_0}
&= \frac{-\frac{1}{z_0}}{1 - \frac{z}{z_0}}
 = -\frac{1}{z_0} \sum_{n=0}^\infty \left(\frac{z}{z_0}\right)^n \\
&= \sum_{n=0}^\infty -\frac{1}{z_0^{n+1}} z^n.
\end{align*}
If $|z| > |z_0|$, then $\left|\frac{z_0}{z}\right| < 1$ so
\begin{align*}
   \frac{1}{z - z_0}
&= \frac{\frac{1}{z}}{1 - \frac{z_0}{z}}
 = \frac{1}{z}
   \sum_{n=0}^\infty
     \left(\frac{z_0}{z}\right)^n \\
&= \sum_{n=0}^\infty
     \frac{z_0^n}{z^{n+1}} \\
&= \sum_{m=-\infty}^{-1} \frac{z^m}{z_0^{m+1}}.
\end{align*}

\end{proof}

To find the Laurent series of
$$
  f(z)
= \frac{1}{(z-1)(z-2)}
= \frac{1}{z - 2} - \frac{1}{z - 1}
$$
and we can then find a Laurent series of $f$
on the annulus $A(0, 1, 2)$.